pcuic/theories/PCUICAst.v
@@ -1,5 +1,5 @@
 (* Distributed under the terms of the MIT license. *)
-From Coq Require Import Morphisms.
+From Coq Require Import ssreflect Morphisms.
 From MetaCoq.Template Require Export utils Universes BasicAst Environment Reflect.
 From MetaCoq.Template Require EnvironmentTyping.
 From MetaCoq.PCUIC Require Export PCUICPrimitive.
@@ -575,7 +575,7 @@ Lemma map_predicate_id x : map_predicate (@id _) (@id term) (@id term) x = id x.
 Proof.
   unfold map_predicate; destruct x; cbn; unfold id.
   f_equal. apply map_id.
-  now rewrite map_decl_id, map_id.
+  now rewrite map_decl_id map_id.
 Qed.
 Hint Rewrite @map_predicate_id : map.
 
@@ -671,6 +671,13 @@ Proof.
 Qed.
 Hint Rewrite map_context_map : map.
 
+Lemma map_map_context {A} (f : context_decl -> A) (g : term -> term) (ctx : context) :
+  map f (map_context g ctx) = map (f ∘ map_decl g) ctx.
+Proof.
+  now rewrite /map_context map_map_compose.
+Qed.
+Hint Rewrite @map_map_context : map.
+
 Lemma map_predicate_id_spec {A} finst (f f' : A -> A) (p : predicate A) :
   finst (puinst p) = puinst p ->
   map f (pparams p) = pparams p ->
@@ -716,7 +723,7 @@ Qed.
 
 Lemma map_fold_context f g ctx : map (map_decl f) (fold_context g ctx) = fold_context (fun i => f ∘ g i) ctx.
 Proof.
-  rewrite !fold_context_alt, map_mapi. 
+  rewrite !fold_context_alt map_mapi. 
   apply mapi_ext => i d. now rewrite compose_map_decl.
 Qed.
 Hint Rewrite map_fold_context : map.
@@ -724,7 +731,7 @@ Hint Rewrite map_fold_context : map.
 Lemma mapi_context_map (f : nat -> term -> term) g (ctx : context) :
   mapi_context f (map g ctx) = mapi (fun i => map_decl (f (Nat.pred #|ctx| - i)) ∘ g) ctx.
 Proof.
-  rewrite mapi_context_fold, fold_context_alt, mapi_map. now len.
+  rewrite mapi_context_fold fold_context_alt mapi_map. now len.
 Qed.
 Hint Rewrite mapi_context_map : map.
  
@@ -732,7 +739,7 @@ Lemma mapi_context_map_context (f : nat -> term -> term) g (ctx : context) :
   mapi_context f (map_context g ctx) = 
   mapi_context (fun i => f i ∘ g) ctx.
 Proof.
-  now rewrite !mapi_context_fold, fold_context_map.
+  now rewrite !mapi_context_fold fold_context_map.
 Qed.
 Hint Rewrite mapi_context_map_context : map.
 
@@ -744,12 +751,12 @@ Proof.
 Qed.
 Hint Rewrite map_context_mapi_context : map.
 
-Lemma map_mapi_context (f : context_decl -> context_decl) (g : nat -> term -> term) (ctx : context) :
+Lemma map_mapi_context {A} (f : context_decl -> A) (g : nat -> term -> term) (ctx : context) :
   map f (mapi_context g ctx) = mapi (fun i => f ∘ map_decl (g (Nat.pred #|ctx| - i))) ctx.
 Proof.
-  now rewrite mapi_context_fold, fold_context_alt, map_mapi.
+  now rewrite mapi_context_fold fold_context_alt map_mapi.
 Qed.
-Hint Rewrite map_mapi_context : map.
+Hint Rewrite @map_mapi_context : map.
 
 Lemma shiftf0 {A B} (f : nat -> A -> B) : shiftf f 0 =2 f.
 Proof. intros x. unfold shiftf. now rewrite Nat.add_0_r. Qed.
@@ -766,7 +773,7 @@ Proof.
   unfold map_predicate, map_predicate_k. destruct p; cbn.
   f_equal.
   now rewrite map_map.
-  now rewrite !mapi_context_fold, fold_context_compose, shiftf0.
+  now rewrite !mapi_context_fold fold_context_compose shiftf0.
   now len.
 Qed.
 Hint Rewrite map_predicate_k_map_predicate_k : map.
@@ -781,7 +788,7 @@ Proof.
   unfold map_predicate, map_predicate_k. destruct p; cbn.
   f_equal.
   apply map_map.
-  rewrite !mapi_context_fold, map_fold_context.
+  rewrite !mapi_context_fold map_fold_context.
   reflexivity.
 Qed.
 Hint Rewrite map_predicate_map_predicate_k : map.
@@ -824,7 +831,7 @@ Proof.
   unfold map_branch, map_branch_k; destruct b; cbn. len.
   f_equal.
   rewrite !mapi_context_fold.
-  now rewrite !fold_context_compose, shiftf0.
+  now rewrite !fold_context_compose shiftf0.
 Qed.
 Hint Rewrite map_branch_k_map_branch_k : map.
 
@@ -837,7 +844,7 @@ Lemma map_branch_map_branch_k
 Proof.
   unfold map_branch, map_branch_k; destruct b; cbn.
   f_equal.
-  now rewrite !mapi_context_fold, map_fold_context.
+  now rewrite !mapi_context_fold map_fold_context.
 Qed.
 
 Hint Rewrite map_branch_map_branch_k : map.
@@ -859,7 +866,7 @@ Hint Rewrite map_branch_k_map_branch : map.
 Lemma map_branch_id x : map_branch (@id term) x = id x.
 Proof.
   unfold map_branch, id; destruct x; cbn.
-  f_equal. now rewrite map_decl_id, map_id.
+  f_equal. now rewrite map_decl_id map_id.
 Qed.
 Hint Rewrite @map_branch_id : map.
 
@@ -916,7 +923,7 @@ Qed.
 Lemma map_context_id (ctx : context) : map_context id ctx = ctx.
 Proof.
   unfold map_context.
-  now rewrite map_decl_id, map_id.
+  now rewrite map_decl_id map_id.
 Qed.
 
 Lemma map_branch_id_spec (f : term -> term) (x : branch term) :
@@ -925,8 +932,8 @@ Lemma map_branch_id_spec (f : term -> term) (x : branch term) :
   map_branch f x = x.
 Proof.
   intros. rewrite (map_branch_eq_spec _ id); auto.
-  now rewrite map_branch_id.
   now rewrite map_context_id.
+  now rewrite map_branch_id.
 Qed.
 Hint Resolve map_branch_id_spec : all.
 
@@ -1087,7 +1094,7 @@ Lemma test_context_k_eq_spec (p q : nat -> term -> bool) k k' {ctx} :
   test_context_k p k ctx = test_context_k q k' ctx.
 Proof.
   intros Hfg <-.
-  induction ctx as [|[na [b|] ty] ctx]; simpl; auto; now rewrite IHctx, Hfg.
+  induction ctx as [|[na [b|] ty] ctx]; simpl; auto; now rewrite IHctx Hfg.
 Qed.
 
 Instance test_context_k_Proper : Proper (`=2` ==> Logic.eq ==> `=1`) (@test_context_k term).
@@ -1180,7 +1187,7 @@ Proof.
   intros [pl [pbod pty]%andb_and]%andb_and.
   rewrite (IHHc pl); simpl.
   unfold test_decl.
-  rewrite (HP _ p0 pty), andb_true_r; simpl.
+  rewrite (HP _ p0 pty) andb_true_r; simpl.
   destruct (decl_body x); simpl in *; eauto.
 Qed.
 
